# ASP: Tutorial 4
# 1. The Einstein relation
> In this exercise, we study the so called Brownian motion of a particle of speed $\vec v$ suspended in a medium of moving smaller particles.
> The particle feels a friction force $\vec f_\gamma$ because of collisions, as well as small kicks $\vec f_c$ from the medium’s particles. Such a particle diffuses with a coefficient $D$ as we will show in the following.
> In 1905, Einstein was able to connect, at thermal equilibrium, this diffusion coefficient to the friction coefficient $\gamma$ as $D=\frac{k_BT}{\gamma}$ $(1.1)$.
> Here we will derive this relation within the framework of Langevin’s 1908 approach in the one dimensional case. The starting point is a stochastic version of Newton’s second law $m\dot v + \gamma v = \xi(t)$ $(1.2)$, where $\xi(t)$ is a stochastic force accounting for the random collisions of the particle with the medium’s particles. To model this force, we take $\xi(t)$ to be a Gaussian white noise with zero mean and covariance $\braket{\xi(t)\xi(t^\prime)}=A\delta(t-t^\prime)$ $(1.3)$ with noise amplitude $A$. As was discussed in the lectures, Brownian motion can be seen as a continuous time limit of the random walk considered in sheet 2, where the particle moves in a random direction at all time $t$.

## a) general solution
> Find the general solution with an arbitrary initial condition $v(0)=v_0$ (your answer should contain a term with an integral involving $\xi(t)$). Show that the term depending on $v_0$ vanishes as $t\rightarrow\infty$.

1. Find partial solution $v_\mathrm{hom}(t)$ of homogeneous differential equation with separation of variables.

$$
\begin{eqnarray}
    m\dot v + \gamma v &=& 0 \\
    \dv{v}{t} &=& -\frac{\gamma}{m} \\
    \frac{\dd v}{v} &=& -\frac{\gamma}{m} \dd{t} \\
    \Rightarrow \int_{v_0}^{v_\mathrm{hom}(t)} \frac{\dd{v}}{v}
        &=& -\frac{\gamma}{m} \int_0^t \dd{t^\prime} \\
    \Rightarrow \ln v_\mathrm{hom}(t) - \ln v_0 &=& -\frac{\gamma}{m} \\
    v_\mathrm{hom}(t) &=& v_0 \exp\left[-\frac{\gamma}{m} t\right] 
\end{eqnarray}
$$

2. variation of parameters:
$$
\begin{eqnarray}
    v(t) &=& v_0(t) \exp\left[-\frac{\gamma}{m} t\right] \\
    \Rightarrow \dot v(t)
        &=& \dot v_0(t) \exp\left[-\frac{\gamma}{m} t\right]
            -\frac{\gamma}{m} v(t) \\
    m\dot v + \gamma v &=& \xi(t) \\
    \Rightarrow
        m\left(
            \dot v_0(t) \exp\left[-\frac{\gamma}{m} t\right]
            -\frac{\gamma}{m} v(t)
        \right)
        + \gamma v(t) &=& \xi(t) \\
    \Leftrightarrow 
        \dot v_0(t)
        &=& \frac{1}{m} \xi(t) \exp\left[\frac{\gamma}{m} t\right] \\
    \Rightarrow v_0(t)
        &=& v_0 + \frac{1}{m} \int_0^t \xi(t^\prime)
            \exp\left[\frac{\gamma}{m} t^\prime\right] \dd{t^\prime} \\
    \Rightarrow v(t)
        &=& 
            \left(
                v_0 + \frac{1}{m} \int_0^t \xi(t^\prime)
                \exp\left[\frac{\gamma}{m} t^\prime\right] \dd{t^\prime}
            \right)
            \exp\left[-\frac{\gamma}{m} t\right] \\
    t\rightarrow\infty
        &\Rightarrow& v_0
            \exp\left[-\frac{\gamma}{m} t\right]
            \rightarrow 0
\end{eqnarray}
$$

The dependency of $v_0$ vanishes for large $t$. This does make sense, since infinitely many interactions create a macrostate for any microstate with $v(0)=v_0$.

## b)
> From now on,we focus on the large time behavior and set $v_0=0$. What is the value of $\braket{v(t)}$? Show that at large $t,t^\prime$ $\braket{v(t)v(t^\prime)}=A(2\gamma m)^{-1} \exp[-\frac{\gamma}{m}|t-t^\prime]$.

At $(1)$, we apply the mean field approximation. Next, we insert $(1.3)$.

$$
\begin{eqnarray}
    \braket{v(t)v(t^\prime)}
        &=& \braket{
                \left(
                    \frac{1}{m} \int_0^t \xi(t^\prime)
                    \exp\left[\frac{\gamma}{m} t^\prime\right] \dd{t^\prime}
                \right)
                \exp\left[-\frac{\gamma}{m} t\right]
            \cdot
                \left(
                    \frac{1}{m} \int_0^{t^\prime} \xi(t^{\prime\prime})
                    \exp\left[\frac{\gamma}{m} t^{\prime\prime}\right]
                    \dd{t^{\prime\prime}}
                \right)
                \exp\left[-\frac{\gamma}{m} t^\prime\right]
            } \\
        &=& \braket{
                \left(
                    \frac{1}{m^2}
                    \int_0^t
                    \int_0^{t^\prime}
                    \xi(t^{\prime\prime\prime})
                    \xi(t^{\prime\prime})
                    \exp\left[\frac{\gamma}{m} (t^{\prime\prime}+t^{\prime\prime\prime})\right]
                    \dd{t^{\prime\prime}}
                \right)
                \exp\left[-\frac{\gamma}{m} (t+t^\prime)\right]
            } \\
     &=&
            \left(
                \frac{1}{m^2}
                \int_0^t
                \int_0^{t^\prime}
                \underbrace{\braket{
                    \xi(t^{\prime\prime\prime})
                    \xi(t^{\prime\prime})
                }}_{A\delta(t^{\prime\prime\prime}-t^{\prime\prime})}
                \exp\left[\frac{\gamma}{m} (t^{\prime\prime}+t^{\prime\prime\prime})\right]
                \dd{t^{\prime\prime}}
                \right)
            \exp\left[-\frac{\gamma}{m} (t+t^\prime)\right]
            \\
        &=&
            \left(
                \frac{1}{m^2}
                \int_0^{\tilde t}
                \exp\left[2\frac{\gamma}{m}t^*\right]
                \dd{t^*}
            \right)
            \exp\left[-\frac{\gamma}{m} (t+t^\prime)\right]
            \\
        &=& \frac{Am}{2\gamma m^2}
            \exp[2\frac{\gamma}{m}\tilde t]
            \exp\left[-\frac{\gamma}{m}(t+t^\prime)\right] \\
        &=& \frac{A}{2\gamma m}
            \exp\left[-\frac{\gamma}{m}(t+t^\prime-2\tilde t)\right]
\end{eqnarray}
$$

Due to applying the $\delta$ function, we integrate either up to $t$ or to $t^\prime$. Thus, $\tilde t$ can be either. Since both cases are valid, the absolute value must be the result for valid times.

$$
\begin{eqnarray}
    t+t^\prime-2\tilde t &=&
        \begin{cases}
            t - t^\prime &: \tilde t = t^\prime \\
            t^\prime - t &: \tilde t = t
        \end{cases} \\
    \Rightarrow t+t^\prime-2\tilde t &\overset{!}{=}& |t-t^\prime|
\end{eqnarray}
$$

## c) Energy
> From the previous question, compute the mean kinetic energy $\frac{1}{2}m\braket{v(t)^2)}$. Compare the result to the classical equipartition theorem and find the value of $A$ at thermal equilibrium. Does the dependence of $A$ on $T$ make sense physically?

$$
\begin{eqnarray}
    \frac{1}{2} m \braket{v(t)^2}
        &=& \frac{1}{2} m \braket{v(t)v(t^\prime)} |_{t=t^\prime} \\
        &=& \frac{1}{2} m \braket{v(t)v(t^\prime)} |_{t=t^\prime} \\
        &=& \frac{1}{2} m \frac{A}{2\gamma m}
            \exp[-\frac{\gamma}{m}|t-t^\prime|] |_{t=t^\prime} \\
        &=& \frac{A}{4\gamma} \\
    \braket{E} &=& \frac{3}{2} k_BT \\
    \Rightarrow \frac{A}{4\gamma}
        &=& \frac{3}{2} k_BT \\
    \Rightarrow A &=& 6k_BT\gamma
\end{eqnarray}
$$

The dependency $A(T)$ makes sense, meaning the amplitude of noise is proportional to temperature. On high temperature, particles move much more around and create more noise. If it's cold, particles move less, hence less noise.

## d) Diffusion
> Confirm that the behavior is indeed diffusive by showing that $\braket{x(t)^2} \rightarrow 2Dt$ and verify that $D$ is given by the Einstein relation. This can be done by integrating the expression you got in c) over $t$ and $t^\prime$.


# 2. Birth-death processes
> Consider a non-negative integer valued random variable $n\in\mathbb N_0$, that represents the population of a given species. A birth-death process is defined as a continuous-time stochastic process described by the master equation $(2.1)$, where $a_n$ and $b_n$ describe the rates at which births and deaths occur, respectively.

$$
\begin{eqnarray}
    \dv{P_n}{t} &=&
        a_{n-1}P_{n-1}
        + b_{n+1}P_{n+1}
        + (a_n+b_n)P_n\hspace{5cm}(2.1)
\end{eqnarray}
$$

We can reach $n$ creatures from a state with $n-1$ creature and $1$ birth, or from $n+1$ creatures and $1$ death. If there are $n$ creatures and either one gets born or dies, the state $n$ is left.

## a) proofs
### a.1 expectation value
$$
\begin{eqnarray}
    \dv{\braket{n}}{t} &=&
        \braket{a_n} - \braket{b_n}\hspace{5cm}(2.2)
\end{eqnarray}
$$

Intuitively, the average change depends on the difference of birth and death rates: If, on average, more (less) creatures are born, the number of creatures rises (drops).
$$
\begin{eqnarray}
    \braket{n} &=& \sum_{n=0}^\infty nP_n \\
    \dv{\braket{n}}{t} &=& \dv{t} \sum_{n=0}^\infty nP_n \\
        &=& \sum_{n=0}^\infty n \dv{P_n}{t} \\
        &=&
            \sum_{n=0}^\infty n a_{n-1}P_{n-1}
            + \sum_{n=0}^\infty n b_{n+1}P_{n+1}
            - \sum_{n=0}^\infty n a_n P_n
            - \sum_{n=0}^\infty n b_n P_n \\
        &=&
            \sum_{n=0}^\infty (n+1) a_nP_n
            + \sum_{n=1}^\infty (n-1) b_n P_n
            - \sum_{n=0}^\infty n a_n P_n
            - \sum_{n=0}^\infty n b_n P_n \\
        &=&
            \underbrace{\sum_{n=0}^\infty a_nP_n}_{\braket{a_n}}
            - \underbrace{\sum_{n=0}^\infty b_nP_n}_{\braket{b_n}}
            \underbrace{
                + \sum_{n=0}^\infty n a_n P_n
                - \sum_{n=0}^\infty n a_n P_n
            }_{0}
            \underbrace{
                + \sum_{n=1}^\infty n b_n P_n
                - \sum_{n=0}^\infty n b_n P_n
            }_{0}  \\
        &=& \braket{a_n} - \braket{b_n} \\
        && \hspace{3cm} \square
\end{eqnarray}
$$

### a.2 variance
$$
\begin{eqnarray}
    \dv{\braket{n^2}}{t} &=&
        2\braket{n(a_n-b_n)} + \braket{a_n+b_n}\hspace{5cm}(2.3)
\end{eqnarray}
$$

proof:
$$
\begin{eqnarray}
    \braket{n^2} &=& \sum_{n=0}^\infty n^2P_n \\
    \dv{\braket{n^2}}{t} &=& \dv{t} \sum_{n=0}^\infty n^2P_n \\
        &=& \sum_{n=0}^\infty n^2 \dv{P_n}{t} \\
        &=&
            \sum_{n=0}^\infty n^2 a_{n-1}P_{n-1}
            + \sum_{n=0}^\infty n^2 b_{n+1}P_{n+1}
            - \sum_{n=0}^\infty n^2 a_n P_n
            - \sum_{n=0}^\infty n^2 b_n P_n \\
        &=&
            \sum_{n=0}^\infty (n+1)^2 a_nP_n
            + \sum_{n=1}^\infty (n-1)^2 b_n P_n
            - \sum_{n=0}^\infty n^2 a_n P_n
            - \sum_{n=0}^\infty n^2 b_n P_n \\
        &=&
            \sum_{n=0}^\infty (\underbrace{n^2}_{*}+2n+1) a_nP_n
            + \sum_{n=1}^\infty (\underbrace{n^2}_{*}-2n+1) b_n P_n
            \underbrace{
                - \sum_{n=0}^\infty n^2 a_n P_n
                - \sum_{n=0}^\infty n^2 b_n P_n
            }_* \\
        &=&
            \sum_{n=0}^\infty (2n+1) a_nP_n (-2n+1) b_n P_n \\
        &=&
            \sum_{n=0}^\infty 2n(a_n-b_n)P_n
            + \sum_{n=0}^\infty (a_n+b_n) P_n \\
        &=&
            2\braket{n(a_n-b_n)} + \braket{a_n+b_n} \\
        && \hspace{6cm} \square
\end{eqnarray}
$$

## b) bacteria growth
> Consider a process in which the size $n$ of a bacterial population changes by cell division $C\rightarrow2C$ and cell death $C\rightarrow0$. The division rate per cell is $r$ and the death rate per cell is $d$, so that the population transitions from $n$ to $n+1$ at rate $r_n$, and from $n$ to $n-1$ at rate $\dd n$. Write down the master equation for the process. Using the result from part a), write down the evolution equations of $\expval{n}$ and $\expval{n^2}$. Solve these equations with the initial condition $P(n)=\delta_{n,n_0}$.

In each step, only a single cell may either divide or die.

$$
\begin{eqnarray}
    \dv{P_n}{t} &=& rn P_{n-1} + dn P_{n+1} - (r+d)nP_n \\
    \Rightarrow \dv{\braket{n}}{t} &=& \braket{rn} - \braket{dn} \\
        &=& (r - d)\braket{n} \\
    \Rightarrow \dv{\braket{n^2}}{t} &=& 2\braket{n^2(r-d)} + \braket{(r+d)n} \\
        &=& 2(r-d)\braket{n^2} + (r+d)\braket{n}
\end{eqnarray}
$$

## c)
> When $r>d$, the population grows without bound. When the density of cells becomes high, we might expect that they start to die because of lack of space or food. This can have an indirect effect on the population or a direct one if cells start to kill each other. In both cases, these effects can be taken into account via pair coalescence where $2C\rightarrow C$ with rate per pair $\lambda$. Explain why this gives a contribution to $b_n$ of the form $b_n = \lambda n(n-1)/2$. Can you still solve $(2.3)$? To make progress, we resort to a mean-field approximation where we neglect all fluctuations by setting $\braket{n^2}=\braket{n}^2$. Show that the resulting equation for $n_{MF}(t)\equiv \braket{n(t)}$ is given by $(2.4)$ and show that there are two possible steady states, which are reached depending on the values of the rates.
$$
\begin{eqnarray}
    \dv{n_{MF}(t)}{t}
        &=& (r-d-\frac{\lambda}{2})n_{MF}(t)
            - \frac{\lambda}{2} n_{MF}^2(t) \hspace{5cm} (2.4)
\end{eqnarray}
$$
> This is an example of a phase transition between an absorbing state (which cannot be escaped once reached) and an active state, where the population is nonzero and fluctuates.

$\lambda$ is the coalescence rate per pair. There are $(n-1)$ possible pairings for each of the $n$ cells, thus $n(n-1)$ times the effect. This rate must be bisected, because only one of those two cells changes. $(2.3)$ can be applied since it is defined for any $b_n$, i.e. without constraints.

$$
\begin{eqnarray}
    \dv{P_n}{t} &=&
        a_{n-1}P_{n-1}
        + b_{n+1}P_{n+1}
        + (a_n+b_n)P_n\hspace{5cm} \\
    a_n &=& r \\
    b_n &=& d + \frac{\lambda n(n-1)}{2} \\
    \dv{\braket{n^2}}{t} &=&
        2\braket{n(a_n-b_n)} + \braket{a_n+b_n} \\
        &=&
            2\braket{n^2(r-d-\frac{\lambda (n-1)}{2})}
            + \braket{(r+d+\frac{\lambda (n-1)}{2})n} \\
        &=& 2(r-d)\braket{n^2} - \lambda\braket{n-1}
            + (r+d)\braket{n}+\frac{\lambda}{2}\braket{(n-1)n} \\
        &=& 2(r-d)n_\mathrm{MF}^2 - \lambda(n_\mathrm{MF}-1)
            + (r+d)n_\mathrm{MF}+\frac{\lambda}{2}(n_\mathrm{MF}-1)n_\mathrm{MF}
\end{eqnarray}
$$

The latter can be motivated by the [[20230223130500|CLT]] or the [[20230223130045|law of large numbers]] since $n\ggg1$. Further, a [[20230228134301|Poisson distribution]] can be assumed. For this, $\braket{n^2}-\braket{n}=\braket{n}$ is valid for any $n$.

$$
\begin{eqnarray}
    \braket{n} &\equiv& n_\mathrm{MF} \\
    \mathrm{CLT}\Rightarrow \braket{n(n-1)} &\approx& n_\mathrm{MF}^2
\end{eqnarray}
$$
